cava/cava/Cava/Arrow/CavaNotation.v
@@ -14,11 +14,12 @@
 (* limitations under the License.                                           *)
 (****************************************************************************)
 
-From Coq Require Import Arith Eqdep_dec List Lia NArith Omega.
+From Coq Require Import Arith Eqdep_dec List Lia NArith Omega String.
 From Arrow Require Import Category Kappa ClosureConversion.
 From Cava Require Import BitArithmetic Arrow.CavaArrow Arrow.CavaExpression.
 
 Import ListNotations.
+Import EqNotations.
 
 Declare Scope kappa_scope.
 Declare Custom Entry expr.
@@ -27,11 +28,17 @@ Delimit Scope kappa_scope with kappa.
 (* Kappa expression and application *)
 
 Module KappaNotation.
-  Notation "<[ e ]>" := (e%kappa) (at level 1, e custom expr at level 1).
+  Notation "<[ e ]>" := (
+    fun (cava: Cava) => 
+    Closure_conversion (object_decidable_equality:=decKind) (Desugar (fun var => e%kappa))
+   ) (at level 1, e custom expr at level 1).
+
+  (* Notation "<[ e ]>" := (e%kappa) (at level 1, e custom expr at level 1). *)
 
   Notation "\ x .. y => e" := (Abs (fun x => .. (Abs (fun y => e)) ..))
-    (in custom expr at level 200, x binder, right associativity,
-    format "'[' \  '/  ' x  ..  y =>  '/  ' e ']'")
+    (in custom expr at level 200, x binder, right associativity
+    (* , format "'[' \  '/  ' x  ..  y =>  '/  ' e ']'" *)
+    )
                                     : kappa_scope.
 
   Notation "x y" := (App x y) (in custom expr at level 3, left associativity) : kappa_scope.
@@ -52,8 +59,8 @@ Module KappaNotation.
 
   (* Escaping *)
 
-  Notation "! x" := (x)(in custom expr at level 2, x global) : kappa_scope.
-  Notation "!( x )" := (x) (in custom expr, x constr) : kappa_scope.
+  Notation "! x" := (Morphism x)(in custom expr at level 2, x global) : kappa_scope.
+  Notation "!( x )" := (Morphism x) (in custom expr, x constr) : kappa_scope.
 
   Notation "( x , .. , y , z )" := (
     (tupleHelper x .. (tupleHelper y z) .. )
@@ -101,11 +108,10 @@ Module KappaNotation.
   Notation "x ++ y" := (App (App (Concat _ _) x) y) (in custom expr at level 4) : kappa_scope.
   Notation "x :: y" := (App (App (Cons _) x) y) (in custom expr at level 4) : kappa_scope.
 
-  Notation "'true'" := (@LiftConstant _ Bit true) (in custom expr at level 2) : kappa_scope.
-  Notation "'false'" := (@LiftConstant _ Bit false) (in custom expr at level 2) : kappa_scope.
+  Notation "'true'" := (LiftConstant Bit true) (in custom expr at level 2) : kappa_scope.
+  Notation "'false'" := (LiftConstant Bit false) (in custom expr at level 2) : kappa_scope.
 
-  Notation "# x" := (@LiftConstant _ (Vector Bit _) x)%N (in custom expr at level 2, x constr at level 4) : kappa_scope.
-
+  Notation "# x" := (LiftConstant (Vector Bit _) x)%N (in custom expr at level 2, x constr at level 4) : kappa_scope.
 
   Notation " v [ x : y ] " :=
         (App (Slice _ x y _ _) v)
@@ -120,11 +126,15 @@ Module KappaNotation.
     (App (App (Snoc _) .. (App (App (Snoc _) EmptyVec) x) ..) y) (in custom expr at level 4) : kappa_scope.
 End KappaNotation.
 
-Notation "'to_arrow' circuit" := (
-  insert_rightmost_tt1 _ >>> 
-  closure_conversion (object_decidable_equality:=decKind) (Desugar (circuit)) (ltac:(simpl;tauto))
-)(at level 100).
+Definition make_module {i o} 
+  (name: string)
+  (expr: forall cava: Cava, i ~[cava]~> o)
+  : forall cava: Cava, i ~[cava]~> o
+  := fun cava => mk_module _ _ name (expr _).
+  (* (Closure_conversion (object_decidable_equality:=decKind) (Desugar expr)). *)
 
+Import KappaNotation.
+Local Open Scope kind_scope.
 
 Section regression_examples.
   Import KappaNotation.
@@ -132,39 +142,41 @@ Section regression_examples.
 
   Context {var: Kind -> Kind -> Type}.
 
-  Definition ex0_constant: CavaExpr var << Vector Bit 10, Unit >> (Vector Bit 8).
-    refine (<[ \x => x [ 7 : 0 ] ]>); lia.
-  Defined.
+  Program Definition ex0_constant: forall cava: Cava, << Vector Bit 10, Unit >> ~> (Vector Bit 8)
+    := <[ \x => x [ 7 : 0 ] ]>.
+  Next Obligation. lia. Qed.
 
-  Definition ex1_constant: CavaExpr var << Bit, Unit >> Bit := <[ \x => true ]>.
-  Definition ex2_parameterized (n: nat): CavaExpr var << Bit, Unit >> Bit :=
+  Definition ex1_constant: forall cava: Cava, << Bit, Unit >> ~> Bit := <[ \x => true ]>.
+  Definition ex2_parameterized (n: nat): forall cava: Cava, << Bit, Unit >> ~> Bit :=
   match n with
   | O => <[ \ x => true ]>
   | S n => <[ \ x => xor x x ]>
   end.
 
-  Definition ex3_to_vec: CavaExpr var << Bit, Unit >> (Vector Bit 1) :=
+  Definition ex3_to_vec: forall cava: Cava, << Bit, Unit >> ~> (Vector Bit 1) :=
   <[ \ x => vector { x } ]>.
-  Definition ex4_index_vec: CavaExpr var << Vector Bit 10, Unit >> Bit :=
+  Definition ex4_index_vec: forall cava: Cava, << Vector Bit 10, Unit >> ~> Bit :=
   <[ \ x => index x (# 1) ]>.
-  Definition ex5_index_vec2: CavaExpr var << Vector Bit 10, Unit >> Bit :=
+  Definition ex5_index_vec2: forall cava: Cava, << Vector Bit 10, Unit >> ~> Bit :=
   <[ \ x => x [# 1] ]>.
-  Definition ex6_concat: CavaExpr var << Vector Bit 2, Bit, Unit >> (Vector Bit 3) :=
+  Definition ex6_concat: forall cava: Cava, << Vector Bit 2, Bit, Unit >> ~> (Vector Bit 3) :=
   <[ \ x v => snoc x v ]>.
-  Definition ex7_xor: CavaExpr var << Bit, Bit, Unit >> Bit :=
+  Definition ex7_xor: forall cava: Cava, << Bit, Bit, Unit >> ~> Bit :=
   <[ \ x y => xor x y ]>.
-  Definition ex7_tupled_destruct: CavaExpr var << << Bit, Bit>>, Unit>> Bit :=
+  Definition ex7_tupled_destruct: forall cava: Cava, << << Bit, Bit>>, Unit>> ~> Bit :=
   <[ \ xy =>
     let '(x,y) = xy in
     y ]>.
-  Definition ex8_multiindex: CavaExpr var << Vector (Vector Bit 5) 10, Unit >> Bit :=
+  Definition ex8_multiindex: forall cava: Cava, << Vector (Vector Bit 5) 10, Unit >> ~> Bit :=
   <[ \ x => x[#0][#1] ]>.
-  Definition ex9_mkvec: CavaExpr var << Bit, Unit >> (Vector Bit 2) :=
+  Definition ex9_mkvec: forall cava: Cava, << Bit, Unit >> ~> (Vector Bit 2) :=
   <[ \x => vector { true, false } ]>.
-  Definition ex10: CavaExpr var << Vector Bit 10, Vector Bit 10, Unit >> (Vector Bit 11) :=
+  Definition ex10: forall cava: Cava, << Vector Bit 10, Vector Bit 10, Unit >> ~> (Vector Bit 11) :=
   <[ \ x y => x + y ]>.
-  Definition ex11: CavaExpr var << Vector Bit 10, Vector Bit 10, Unit >> (Vector Bit 10) :=
+  Definition ex11: forall cava: Cava, << Vector Bit 10, Vector Bit 10, Unit >> ~> (Vector Bit 10) :=
   <[ \ x y => x +% y ]>.
+  Definition ex12_module: forall cava: Cava, <<Vector Bit 10, Unit>> ~> Vector Bit 10
+    := make_module "ex12_module" <[ \x => x +% x ]>.
 
   Fixpoint copy_object_pow2 o (n:nat): Kind :=
   match n with
@@ -175,9 +187,9 @@ Section regression_examples.
   Fixpoint tree
     (A: Kind)
     (n: nat)
-    (f: CavaExpr var << A, A, Unit >> A)
+    (f: forall (cava: Cava), << A, A, Unit >> ~[cava]~> A)
     {struct n}
-    : CavaExpr var << copy_object_pow2 A n, Unit >> A :=
+    : forall cava: Cava, << copy_object_pow2 A n, Unit >> ~> A :=
   match n with
   | O => <[ \ x => x ]>
   | S n' =>
@@ -188,8 +200,21 @@ Section regression_examples.
     ]>
   end.
 
+  Definition add' (n: nat)
+    : forall cava: Cava, <<Vector Bit n, Vector Bit n, Unit>> ~> (Vector Bit n)
+    := 
+    match Nat.eq_dec (Init.Nat.max n n) n with
+    | left Heq => rew [fun x => forall cava: Cava, _~>Vector Bit x] Heq in <[\x y=> x +% y]>
+    | right Hneq => (ltac:(lia))
+    end.
+
+  Definition adder_tree
+    (bitsize n: nat)
+    : forall cava:Cava, <<copy_object_pow2 (Vector Bit bitsize) n, Unit>> ~> (Vector Bit bitsize) :=
+    tree (Vector Bit bitsize) n (add' bitsize).
+
   Definition xilinxFullAdder
-    : CavaExpr var << Bit, << Bit, Bit >>, Unit>> (Tuple Bit Bit) :=
+    : forall cava: Cava, << Bit, << Bit, Bit >>, Unit>> ~> (Tuple Bit Bit) :=
     <[ \ cin ab =>
       let a = fst ab in
       let b = snd ab in
@@ -198,10 +223,5 @@ Section regression_examples.
       let cout     = muxcy part_sum (cin, a) in
       (sum, cout)
     ]>.
-
-  Definition adder_tree
-    (bitsize n: nat)
-    : CavaExpr var <<copy_object_pow2 (Vector Bit bitsize) n, Unit>> (Vector Bit bitsize) :=
-    tree (Vector Bit bitsize) n (UnsignedAdd _ _ _).
 
 End regression_examples.
